finished progress and preservation for full calc, excepting choice operator

FiatFormal/Language/Exp.v
@@ -37,6 +37,59 @@ Fixpoint dcOfAlt (aa: alt) : datacon :=
  end.
 Hint Unfold dcOfAlt.
 
+(* Get the alternative body that matches a given constructor. *)
+Fixpoint getAlt (dc: datacon) (alts: list alt) {struct alts}
+                : option alt :=
+ match alts with
+ |  nil  => None
+
+ |  AAlt dc' tsArgs x :: alts'
+ => if datacon_beq dc dc'
+     then Some (AAlt dc' tsArgs x)
+     else getAlt dc alts'
+ end.
+
+(* If we get a single alternative from a list,  *)
+(*    then that alternative was in the list. *)
+Lemma getAlt_in
+ :  forall dc alt alts
+ ,  getAlt dc alts = Some alt
+ -> In alt alts.
+Proof.
+ intros.
+ induction alts.
+  false.
+  destruct a as [dc' tsArgs x].
+  simpl in H.
+  breaka (datacon_beq dc dc').
+   inverts H.
+   apply datacon_beq_eq in HeqX; auto.
+Qed.
+
+(* Given a data constructor, if one of the alternatives in a  *)
+(*    list matches that data constructor then we can get the other *)
+(*    information about the alternative from the list. *)
+Lemma getAlt_exists
+ :  forall d alts
+ ,  In d (map dcOfAlt alts)
+ -> (exists tsArgs x, getAlt d alts = Some (AAlt d tsArgs x)).
+Proof.
+ intros.
+ induction alts.
+  simpl in H. false.
+  simpl in H. inverts H.
+   destruct a. simpl.
+   breaka (datacon_beq d d).
+    exists l. exists e. auto.
+    apply datacon_beq_false in HeqX. false.
+   lets D: IHalts H0.
+   destruct a. simpl.
+    breaka (datacon_beq d d0).
+     apply datacon_beq_eq in HeqX. subst. auto.
+     exists l. exists e. auto.
+Qed.
+
+
 (********************************************************************)
 (* Mutual induction principle for expressions.
    As expressions are indirectly mutually recursive with lists,
@@ -445,6 +498,16 @@ with substXA (d: nat) (u: exp) (a: alt) : alt :=
        match a with
        | AAlt dc ts x => AAlt dc ts (substXX (d + length ts) (liftXX (length ts) 0 u) x)
        end.
+
+Fixpoint substXXs (d: nat) (us: list exp) (xx: exp) :=
+ match us with
+ | nil      => xx
+ | u :: us' => substXXs d us'
+                 (substXX d (liftXX (List.length us') 0 u)
+                            xx)
+ end.
+
+
 
 (* The data constructor of an alternative is unchanged
    by lifting. *)
