FiatFormal/Language/Step.v
@@ -3,37 +3,136 @@ Require Import FiatFormal.Language.SubstTypeExp.
 Require Import FiatFormal.Language.SubstExpExp.
 Require Export FiatFormal.Language.Exp.
 
+Require Export FiatFormal.Language.Context.
 
-(* Small step expression evaluation *)
+(* TODO: consider implications of below definition...
+         esp. that nary function application requires
+         value of function but only wnfX of args *)
+
+(*  Evaluation contexts for expressions.
+    This describes a place in the exp AST where the sub-expression
+    there is able to take an evaluation step *)
+Inductive exp_ctx : (exp -> exp) -> Prop :=
+
+ (* Left of an application *)
+ | XcApp1
+   : forall x2,
+     exp_ctx (fun xx => XApp xx x2)
+
+ (* The right of an application can step only when the left is
+    already a value. *)
+ | XcApp2
+   : forall v1,
+     value v1
+     -> exp_ctx (fun xx => XApp v1 xx)
+
+ | XcCon
+   : forall dc C,
+     exps_ctx wnfX C
+     -> exp_ctx (fun xx => XCon dc (C xx))
+
+ (* We need to reduce the discriminant of a match to a value. *)
+ | XcMatch
+   : forall alts,
+     exp_ctx (fun xx => XMatch xx alts)
+
+ | XcTup
+   : forall C,
+     exps_ctx wnfX C
+     -> exp_ctx (fun xx => XTup (C xx))
+
+ | XcProj
+   : forall n,
+     exp_ctx (fun xx => XProj n xx)
+
+ | XcNApp1
+   : forall xs,
+     exp_ctx (fun xx => XNApp xx xs)
+
+ | XcNApp2
+   : forall v1 C,
+     value v1
+     -> exps_ctx wnfX C
+     -> exp_ctx (fun xx => XNApp v1 (C xx)).
+
+Hint Constructors exp_ctx.
+
 Inductive STEP : exp -> exp -> Prop :=
-  (* value applications *)
-  | ESLamApp
-    :  forall t11 x12 v2
-    ,  value v2
-    -> STEP (XApp (XLam t11 x12) v2) (substXX 0 v2 x12)
+ (* Step some sub-expression in an evaluation context *)
+ | EsContext
+   : forall C x x',
+     exp_ctx C
+     -> STEP x x'
+     -> STEP (C x) (C x')
 
-  | ESApp1
-    :  forall x1 x1' x2
-    ,  STEP x1 x1'
-    -> STEP (XApp x1 x2) (XApp x1' x2)
+ (* Function application. *)
+ | EsLamApp
+   : forall t11 x12 v2,
+     wnfX v2
+     -> STEP (XApp (XLam t11 x12) v2)
+            (substXX 0 v2 x12)
 
-  | ESApp2
-    :  forall v1 x2 x2'
-    ,  value v1
-    -> STEP x2 x2'
-    -> STEP (XApp v1 x2) (XApp v1 x2')
+ | EsFixApp
+   : forall t11 t22 x12 v2,
+     wnfX v2
+     -> STEP (XApp (XFix t11 t22 x12) v2)
+            (substXX 0 (XFix t11 t22 x12) (substXX 0 v2 x12))
 
-  (* type applications *)
-  (* | ESLAMAPP *)
-  (*   :  forall x12 t2 *)
-  (*   ,  STEP (XAPP (XLAM x12) t2) (substTX 0 t2 x12) *)
+ | EsTupProj
+   : forall vs n v',
+     Forall wnfX vs
+     -> get n vs = Some v'
+     -> STEP (XProj n (XTup vs)) v'
 
-  (* | ESAPP1 *)
-  (*   :  forall x1 x1' t2 *)
-  (*   ,  STEP x1 x1' *)
-  (*   -> STEP (XAPP x1 t2) (XAPP x1' t2) *).
+ | EsNFunApp
+   : forall x vs ts,
+     Forall wnfX vs
+     -> STEP (XNApp (XNFun ts x) vs)
+            (substXXs 0 vs x)
+
+ (* Match branching. *)
+ | EsMatchAlt
+   : forall dc ts vs alts x,
+     Forall wnfX vs
+     -> getAlt dc alts = Some (AAlt dc ts x)
+     -> STEP (XMatch (XCon dc vs) alts)
+            (substXXs 0 vs x).
 
 Hint Constructors STEP.
+
+Lemma step_context_XCon_exists
+ :  forall  C x dc
+ ,  exps_ctx wnfX C
+ -> (exists x', STEP x x')
+ -> (exists x', STEP (XCon dc (C x)) (XCon dc (C x'))).
+Proof.
+ intros C x dc HC HS.
+ shift x'.
+ eapply (EsContext (fun xx => XCon dc (C xx))); auto.
+Qed.
+
+Lemma step_context_XTup_exists
+  : forall C x,
+    exps_ctx wnfX C
+    -> (exists x', STEP x x')
+    -> (exists x', STEP (XTup (C x)) (XTup (C x'))).
+Proof.
+ intros C x HC HS.
+ shift x'.
+ eapply (EsContext (fun xx => XTup (C xx))); auto.
+Qed.
+
+(* Lemma step_context_XNApp_exists *)
+(*   : forall C x xx ts, *)
+(*     exps_ctx wnfX C *)
+(*     -> (exists x', STEP x x') *)
+(*     -> (exists x', STEP (XNApp (XNFun ts xx) (C x)) (XNApp (XNFun ts xx) (C x'))). *)
+(* Proof. *)
+(*  intros C x xx ts HC HS. *)
+(*  shift x'. *)
+(*  eapply (EsContext (fun xx' => XNApp (XNFun ts xx) (C xx'))); eauto. *)
+(*  apply XcNApp2; eauto. constructor; eauto.  *)
+(* Qed. *)
 
 (* Small step program evaluation *)
 Inductive STEPP : prog -> prog -> Prop :=
@@ -83,25 +182,25 @@ Hint Constructors STEPS.
    context. They're all trivial.
    TODO: Define contexts directly like in the Simple proof.
  *)
-Lemma steps_app1
- :  forall x1 x1' x2
- ,  STEPS x1 x1'
- -> STEPS (XApp x1 x2) (XApp x1' x2).
-Proof.
- intros. induction H; eauto.
-Qed.
-Hint Resolve steps_app1.
+(* Lemma steps_app1 *)
+(*  :  forall x1 x1' x2 *)
+(*  ,  STEPS x1 x1' *)
+(*  -> STEPS (XApp x1 x2) (XApp x1' x2). *)
+(* Proof. *)
+(*  intros. induction H; eauto. *)
+(* Qed. *)
+(* Hint Resolve steps_app1. *)
 
 
-Lemma steps_app2
- :  forall v1 x2 x2'
- ,  value v1
- -> STEPS x2 x2'
- -> STEPS (XApp v1 x2) (XApp v1 x2').
-Proof.
- intros. induction H0; eauto.
-Qed.
-Hint Resolve steps_app2.
+(* Lemma steps_app2 *)
+(*  :  forall v1 x2 x2' *)
+(*  ,  value v1 *)
+(*  -> STEPS x2 x2' *)
+(*  -> STEPS (XApp v1 x2) (XApp v1 x2'). *)
+(* Proof. *)
+(*  intros. induction H0; eauto. *)
+(* Qed. *)
+(* Hint Resolve steps_app2. *)
 
 
 (* Lemma steps_APP1 *)
