FiatFormal/Language/Preservation.v
@@ -5,52 +5,232 @@ Require Import FiatFormal.Language.SubstTypeExp.
 Require Import FiatFormal.Language.SubstTypeType.
 Require Import FiatFormal.Language.TyJudge.
 
-
-(* When an expression takes a step the results has the same type. *)
-Theorem preservation
- :  forall ke te x x' t
- ,  TYPE ke te x t
- -> STEP x x'
- -> TYPE ke te x' t.
+(* The body of an alternative is well typed under an environment
+   that includes the arguments of the constructor being matched. *)
+Lemma getAlt_bodyIsWellTyped_fromAlts
+  : forall ds ke te tPat tResult alts dc tsArgs x,
+    Forall (fun a => TYPEA ds ke te a tPat tResult) alts
+    -> In (AAlt dc tsArgs x) alts
+    -> TYPE ds ke (te >< tsArgs) x tResult.
 Proof.
- intros ke te x x' t HT HS.
- gen ke te x' t.
- induction x; intros.
+ intros.
+ nforall. spec H H0.
+ invert_exp_type. auto.
+Qed.
 
- Case "XVar".
-  inverts HS.
 
- (* Case "XLAM". *)
- (*  inverts HS. *)
+(* The body of an alternative of a case expression is well typed
+   under an environment that includes the arguments of the constructor
+   being matched. *)
+Lemma getAlt_bodyIsWellTyped_fromMatch
+  : forall ds ke te tResult tCon alts dc tsArgs x1 x2,
+    TYPE ds ke te (XMatch x1 alts) tResult
+    -> getDataDef dc ds   = Some (DefData dc tsArgs tCon)
+    -> getAlt     dc alts = Some (AAlt    dc tsArgs x2)
+    -> TYPE ds ke (te >< tsArgs) x2 tResult.
+Proof.
+ intros.
+ inverts keep H.
+ lets HA:  getAlt_in H1.
+ lets HXT: getAlt_bodyIsWellTyped_fromAlts H5 HA.
+ auto.
+Qed.
 
- (* Case "XAPP". *)
- (*  inverts HT. *)
- (*  inverts keep HS. *)
 
-  (* SCase "ESAPPLAM". *)
-  (*  inverts H3. *)
-  (*  eapply subst_type_value in H4; eauto. *)
-  (*  rewrite substTE_liftTE in H4. auto. *)
+(* If an alternative is well typed then the types of the ctor
+   args embedded in it match those in the data type definition *)
+Lemma getAlt_ctorArgTypesMatchDataDef
+  : forall ds ke te tCon tResult alts dc x tsArgs tsArgs',
+    Forall (fun alt => TYPEA ds ke te alt tCon tResult) alts
+    -> getDataDef dc ds = Some (DefData dc tsArgs  tCon)
+    -> getAlt dc alts   = Some (AAlt    dc tsArgs' x)
+    -> tsArgs = tsArgs'.
+Proof.
+ intros. nforall.
+ lets D: getAlt_in H1. spec H D.
+ invert_exp_type.
+ rewrite H0 in H5. inversion H5; auto.
+Qed.
 
-  (* SCase "ESAPP1". *)
-  (*  apply TYAPP; eauto. *)
 
- Case "XLam".
-  inverts HS.
+Lemma liftXX_closed :
+  forall ds te x t n,
+    TYPE ds nil te x t
+    -> length te = n
+    -> x = liftXX 1 n x.
+Proof.
+  intros. gen ds te t n.
+  induction x using exp_mutind
+    with (PA := fun a => forall ds te tBuilds tRes n,
+                    TYPEA ds nil te a tBuilds tRes
+                    -> length te = n
+                    -> a = liftXA 1 n a);
+    intros; try inverts H; nope; simpl.
 
- Case "XApp".
-  inverts HT.
-  inverts keep HS.
+  Case "XVar".
+  lift_cases. exfalso. eapply get_above_false.
+  rewrite <- H0 in l. eauto. eauto. reflexivity.
+  Case "XLam".
+  spec IHx H8. rewrite <- IHx; auto. simpl; auto.
+  Case "XApp".
+  erewrite <- IHx1; eauto.
+  erewrite <- IHx2; eauto.
+  Case "XTup".
+  invert_exp_type.
+  f_equal. (* erewrite <- H2; eauto. *)
+  assert (x = liftXX 1 n x).
+  assert (In x (l0 :> x)) by auto.
+  pose proof (Forall2_exists_left _ _ _ _ H H7).
+  dest y. spec H2 H0. spec H2 H1. auto.
+  rewrite <- H.
 
-  SCase "ESAppLam".
-   inverts H3.
-   lets D: subst_value_value H9 H5. auto.
+  assert (l0 = map (liftXX 1 n) l0).
+  nforall. assert (map (fun b => b) l0 = l0).
+  rewrite <- map_id. auto. rewrite <- H0.
+  rewrite map_map.
+  apply map_ext_in; intros.
+  spec H3 H4.
+  apply in_cons with (a:=x) in H4.
+  pose proof (Forall2_exists_left _ _ _ _ H4 H7).
+  destruct H5.
+  eapply H3; eauto.
+  rewrite <- H0; auto.
 
-  SCase "EsApp1".
-   eapply TYApp; eauto.
+  Case "XProj".
+  assert (x = liftXX 1 n0 x).
+  eapply IHx; eauto. rewrite <- H; auto.
 
-  SCase "EsApp2".
-   eapply TYApp; eauto.
+  Case "XNFun".
+  assert (x = liftXX 1 (n + length ts) x).
+  eapply IHx; eauto. rewrite app_length.
+  burn. burn.
+
+  Case "XNApp".
+  invert_exp_type.
+  assert (x = liftXX 1 n x).
+  eapply IHx; eauto. rewrite <- H; auto.
+  invert_exp_type.
+  assert (x = liftXX 1 n x).
+  eapply IHx; eauto. rewrite <- H; auto.
+  nforall.
+  assert (In x0 (l0 :> x0)) by auto.
+  pose proof (Forall2_exists_left _ _ _ _ H0 H10).
+  dest y. assert (x0 = liftXX 1 n x0) by eauto.
+  rewrite <- H5.
+  assert (l0 = map (liftXX 1 n) l0).
+
+  assert (map (fun b => b) l0 = l0).
+  rewrite <- map_id. auto. rewrite <- H6.
+  rewrite map_map.
+  apply map_ext_in; intros.
+  spec H3 H7.
+  assert (In a (l0 :> x0)) by auto.
+  pose proof (Forall2_exists_left _ _ _ _ H9 H10).
+  destruct H11. eapply H3; eauto.
+  rewrite <- H6; auto.
+
+  Case "XFix".
+  assert (x = liftXX 1 (S (S n)) x).
+  eapply IHx. eauto. rewrite <- H0. auto.
+  rewrite <- H; auto.
+
+  Case "XCon".
+  invert_exp_type.
+  assert (x = liftXX 1 n x).
+  assert (In x (l0 :> x)) by auto.
+  pose proof (Forall2_exists_left _ _ _ _ H H13).
+  dest y. eapply H2; eauto. rewrite <- H.
+  repeat nforall.
+  assert (l0 = map (liftXX 1 n) l0).
+
+  assert (map (fun b => b) l0 = l0).
+  rewrite <- map_id. auto. rewrite <- H0.
+  rewrite map_map.
+  apply map_ext_in; intros.
+  spec H3 H4.
+  assert (In a (l0 :> x)) by auto.
+  pose proof (Forall2_exists_left _ _ _ _ H8 H13).
+  destruct H9. eapply H3; eauto.
+  rewrite <- H0; auto.
+
+  Case "XMatch".
+  invert_exp_type.
+  assert (x = liftXX 1 n x).
+  eapply IHx; eauto. rewrite <- H.
+  repeat nforall.
+  rename x0 into a.
+  assert (a = liftXA 1 n a).
+  assert (In a (l0 :> a)) by auto.
+  spec H6 H0. eapply H2; eauto.
+  rewrite <- H0.
+  assert (l0 = map (liftXA 1 n) l0).
+
+  assert (map (fun b => b) l0 = l0).
+  rewrite <- map_id. auto. rewrite <- H4.
+  rewrite map_map.
+  apply map_ext_in; intros.
+  spec H3 H8.
+  assert (In a0 (l0 :> a)) by auto.
+  spec H6 H9. eapply H3; eauto. rewrite <- H4; auto.
+
+  Case "AAlt".
+  assert (x = liftXX 1 (n + length ts) x).
+  eapply IHx; eauto. rewrite <- H0.
+  rewrite app_length. burn. rewrite <- H; auto.
+Qed.
+
+
+(* When a well typed expression transitions to the next state *)
+(*    then its type is preserved. *)
+Theorem preservation
+  : forall ds x x' t,
+    TYPE ds nil nil x t
+    -> STEP x x'
+    -> TYPE ds nil nil x' t.
+Proof.
+ intros ds x x' t HT HS. gen ds t.
+ induction HS; intros; invert_exp_type; eauto.
+
+ (* Evaluation in an arbitrary context. *)
+ Case "EsContext".
+ destruct H; invert_exp_type; eauto.
+
+ SCase "XCon".
+ eapply TYCon; eauto.
+ eapply exps_ctx_Forall2_swap. eauto. (* why can't this be sequenced? *)
+ apply IHHS. auto.
+
+ SCase "Tup".
+ eapply TYTup; eauto.
+ eapply exps_ctx_Forall2_swap. eauto. (* why can't this be sequenced? *)
+ apply IHHS. auto.
+
+ SCase "NApp".
+ eapply TYNApp; eauto.
+ eapply exps_ctx_Forall2_swap. eauto. (* why can't this be sequenced? *)
+ apply IHHS. auto.
+
+ Case "EsLamApp".
+ eapply subst_value_value; eauto.
+
+ Case "EsFixApp".
+ eapply subst_value_value; eauto.
+ eapply subst_value_value; eauto.
+ assert (v2 = liftXX 1 0 v2).
+ eapply liftXX_closed; eauto.
+ rewrite H0.
+ apply type_tyenv_weaken; auto.
+ eapply (Forall2_get_get_same); eauto.
+
+ Case "EsNFunApp".
+ eapply subst_exp_exp_list; eauto.
+
+ Case "EsCaseAlt".
+ eapply subst_exp_exp_list; eauto.
+ eapply getAlt_bodyIsWellTyped_fromMatch; eauto.
+ (* assert (tsArgs = tsArgs0). *)
+ lets D: getAlt_ctorArgTypesMatchDataDef H4 H7 H0. auto.
+ subst. auto.
 Qed.
 
 
@@ -58,10 +238,10 @@ Qed.
    then the result has the same type as the original.
  *)
 Lemma preservation_steps
- :  forall x1 t1 x2
- ,  TYPE nil nil x1 t1
- -> STEPS x1 x2
- -> TYPE nil nil x2 t1.
+  : forall ds x1 t1 x2,
+    TYPE ds nil nil x1 t1
+    -> STEPS x1 x2
+    -> TYPE ds nil nil x2 t1.
 Proof.
  intros.
  induction H0; eauto.
@@ -74,10 +254,10 @@ Qed.
    Using the left-linearised form for the evaluation.
  *)
 Lemma preservation_stepsl
- :  forall x1 t1 x2
- ,  TYPE nil nil x1 t1
- -> STEPSL x1 x2
- -> TYPE nil nil x2 t1.
+  : forall ds x1 t1 x2,
+    TYPE ds nil nil x1 t1
+    -> STEPSL x1 x2
+    -> TYPE ds nil nil x2 t1.
 Proof.
  intros.
  induction H0.
