FiatFormal/Language/PreservationP.v
@@ -10,19 +10,19 @@ Require Import FiatFormal.Language.Preservation.
 
 (* When a closed program takes a step the result has the same type. *)
 Theorem preservationP
- :  forall p p' t
- ,  TYPEPROG nil nil p t
+ :  forall ds p p' t
+ ,  TYPEPROG ds nil nil p t
  -> STEPP p p'
- -> TYPEPROG nil nil p' t.
+ -> TYPEPROG ds nil nil p' t.
 Proof.
-  intros p p' t HT HS.
-  gen p' t.
+  intros ds p p' t HT HS.
+  gen ds p' t.
   induction p; intros.
   Case "PLet".
   invert HS; intros.
   invert HT; intros; subst.
   invert H; intros; subst.
-  eapply subst_ADT_prog; invert H6; intros; subst.
+  eapply subst_ADT_prog; invert H7; intros; subst.
   simpl in *. eassumption.
   eassumption.
   assumption.
@@ -30,7 +30,7 @@ Proof.
   invert HS; intros; subst.
   invert HT; intros; subst.
   apply TYExp.
-  apply (preservation _ _ _ _ _ H3 H0).
+  apply (preservation _ _ _ _ H4 H0).
 Qed.
 
 
@@ -38,10 +38,10 @@ Qed.
    then the result has the same type as the original.
  *)
 Lemma preservation_steps
- :  forall x1 t1 x2
- ,  TYPE nil nil x1 t1
- -> STEPS x1 x2
- -> TYPE nil nil x2 t1.
+  : forall ds x1 t1 x2,
+    TYPE ds nil nil x1 t1
+    -> STEPS x1 x2
+    -> TYPE ds nil nil x2 t1.
 Proof.
  intros.
  induction H0; eauto.
@@ -54,10 +54,10 @@ Qed.
    Using the left-linearised form for the evaluation.
  *)
 Lemma preservation_stepsl
- :  forall x1 t1 x2
- ,  TYPE nil nil x1 t1
- -> STEPSL x1 x2
- -> TYPE nil nil x2 t1.
+  : forall ds x1 t1 x2,
+    TYPE ds nil nil x1 t1
+    -> STEPSL x1 x2
+    -> TYPE ds nil nil x2 t1.
 Proof.
  intros.
  induction H0.
