FiatFormal/Language/Progress.v
@@ -5,70 +5,291 @@ Require Import FiatFormal.Language.SubstTypeExp.
 Require Import FiatFormal.Language.SubstTypeType.
 Require Import FiatFormal.Language.TyJudge.
 
-
-(* A well typed expression is either a value, or can take a step. *)
-Theorem progress
- :  forall x
- ,  (exists t, TYPE nil nil x t)
- -> value x \/ (exists x', STEP x x') \/ hasChoiceX x.
+Lemma canonicalFormTFun :
+  forall ds ke te t1 t2 x,
+    TYPE ds ke te x (TFun t1 t2)
+    -> value x
+    -> exists x', (x = (XLam t1 x') \/ x = (XFix t1 t2 x')).
 Proof.
- intros.
- induction x; destruct H as [tx].
+  intros. gen ds ke te t1 t2 H0.
+  induction x using exp_mutind
+    with (PA := fun a => a = a); rip; try inverts H0; try nope; try inverts H.
+  exists x; left; reflexivity.
+  exists x; right; reflexivity.
+Qed.
 
- Case "XVar".
-  inverts H. false.
+Lemma canonicalFormTNFun :
+  forall ds ke te tsArgs tRes x,
+    TYPE ds ke te x (TNFun tsArgs tRes)
+    -> value x
+    -> exists x', x = (XNFun tsArgs x').
+Proof.
+  intros. gen ds ke te tsArgs tRes H0.
+  induction x using exp_mutind
+    with (PA := fun a => a = a); rip; try inverts H0; try nope; try inverts H.
+  exists x; reflexivity.
+Qed.
 
- (* Case "XLAM". *)
- (*  left. apply type_wfX in H. auto. *)
+Lemma canonicalFormTNProd :
+  forall ds ke te ts x,
+    TYPE ds ke te x (TNProd ts)
+    -> value x
+    -> exists xs, x = (XTup xs).
+Proof.
+  intros. gen ds ke te ts H0.
+  induction x using exp_mutind
+    with (PA := fun a => a = a); rip; try inverts H0; try nope; try inverts H.
+  exists (@nil exp); reflexivity.
+  exists (l0 :> x); reflexivity.
+Qed.
 
- (* Case "XAPP". *)
- (*  inverts H. *)
- (*  destruct IHx. eauto. *)
- (*  SCase "x value". *)
- (*   right. inverts H. inverts H4. *)
- (*    inverts H1. false. *)
- (*    inverts H0. *)
- (*    exists (substTX 0 t x1). eapply ESLAMAPP. *)
- (*    inverts H0. *)
- (*  SCase "x steps". *)
- (*   right. *)
- (*    destruct H as [x']. *)
- (*    exists (XAPP x' t). *)
- (*    apply ESAPP1. auto. *)
+Lemma wellTypedProjHasX :
+  forall ds ke te ts t xs n,
+    TYPE ds ke te (XTup xs) (TNProd ts)
+    -> get n ts = Some t
+    -> exists x, get n xs = Some x.
+Proof.
+  intros.
+  inverts H.
+  pose proof @get_length_less_exists exp.
+  pose proof(Forall2_length _ _ _ H6).
+  apply get_length_less in H0. rewrite <- H1 in H0.
+  spec H H0. dest x. eauto.
+Qed.
+
+
+(* A well typed expression is either a value, can take a step,
+   or contains a choice. *)
+Theorem progress
+  : forall ds x,
+    (exists t, TYPE ds nil nil x t)
+    -> value x \/ (exists x', STEP x x') \/ hasChoiceX x.
+Proof.
+(*  intros. gen ds. *)
+(*  induction x using exp_mutind *)
+(*    with (PA := fun a => a = a); *)
+(*    rip; first [destruct H as [tx] | destruct H0 as [tx]]. *)
+
+(*  Case "XVar". *)
+(*   inverts H. false. *)
+
+(*  (* Case "XLAM". *) *)
+(*  (*  left. apply type_wfX in H. auto. *) *)
+
+(*  (* Case "XAPP". *) *)
+(*  (*  inverts H. *) *)
+(*  (*  destruct IHx. eauto. *) *)
+(*  (*  SCase "x value". *) *)
+(*  (*   right. inverts H. inverts H4. *) *)
+(*  (*    inverts H1. false. *) *)
+(*  (*    inverts H0. *) *)
+(*  (*    exists (substTX 0 t x1). eapply ESLAMAPP. *) *)
+(*  (*    inverts H0. *) *)
+(*  (*  SCase "x steps". *) *)
+(*  (*   right. *) *)
+(*  (*    destruct H as [x']. *) *)
+(*  (*    exists (XAPP x' t). *) *)
+(*  (*    apply ESAPP1. auto. *) *)
+
+(*  Case "XLam". *)
+(*   left. apply type_wfX in H. auto. *)
+
+(*  Case "XApp". *)
+(*   right. *)
+(*   inverts H. *)
+(*   destruct (IHx1 ds) as [| []]; eauto. *)
+(*   SCase "x1 value". *)
+(*   pose proof (canonicalFormTFun). *)
+(*   spec H0 H5. spec H0 H. *)
+(*   destruct H0 as [x' [LAM | FIX]]; subst. *)
+(*   destruct (IHx2 ds) as [| []]; eauto. *)
+(*   SSCase "x2 value". *)
+(*   left. exists (substXX 0 x2 x'); apply EsLamApp; inverts H0; auto. *)
+(*   SSCase "x2 steps". *)
+(*   destruct H0 as [x'']. *)
+(*   left. exists (XApp (XLam t11 x') x''). eauto. *)
+(*   SSCase "x2 hasChoice". *)
+(*   inversion H0. *)
+(*   destruct (IHx2 ds) as [| []]; eauto. *)
+(*   left. exists (substXX 0 (XFix t11 tx x') (substXX 0 x2 x')). apply EsFixApp; inverts H0; auto. *)
+(*   destruct H0 as [x'']. *)
+(*   left; exists (XApp (XFix t11 tx x') x''). eauto. *)
+(*   inversion H0. *)
+(*   SCase "x1 steps". *)
+(*   left. destruct H as [x1']. exists (XApp x1' x2). apply EsContext. *)
+(*   apply ESApp1; auto. *)
+
+(*   SCase "x1 hasChoice". *)
+(*   inversion H. *)
+(* Qed. *)
+
+
+(* Theorem progress *)
+(*  :  forall ds x t *)
+(*  ,  TYPE ds nil x t *)
+(*  -> value x \/ (exists x', STEP x x'). *)
+(* Proof. *)
+ intros. gen ds.
+ induction x using exp_mutind with
+     (PA := fun a => a = a);
+   rip; first [destruct H as [tx] | destruct H0 as [tx]];
+     try invert_exp_type; nope.
 
  Case "XLam".
-  left. apply type_wfX in H. auto.
+ left; eauto.
 
  Case "XApp".
-  right.
-  inverts H.
-  destruct IHx1 as [| []]; eauto.
-  SCase "x1 value".
-  destruct IHx2 as [| []]; eauto.
+ right.
+ edestruct IHx1; eauto.
+ SCase "value x1".
+ edestruct IHx2; eauto.
+ SSCase "value x2".
+ pose proof (canonicalFormTFun).
+ spec H1 H5. spec H1 H. destruct H1 as [x' [LAM | FIX]]; subst.
+ SSSCase "lam".
+ left; exists (substXX 0 x2 x'). apply EsLamApp. inverts H0; auto.
+ SSSCase "fix".
+ left; exists (substXX 0 (XFix t11 tx x') (substXX 0 x2 x')). apply EsFixApp. inverts H0; auto.
+ destruct H0 as [STx2 | HCx2].
+ SSCase "x2 steps".
+ destruct STx2 as [x2'].
+ left; exists (XApp x1 x2'). auto.
+ SSCase "x2 hasChoice".
+ nope.
+ destruct H as [STx1 | HCx1].
+ SCase "x1 steps".
+ destruct STx1 as [x1'].
+ left; exists (XApp x1' x2).
+ eapply (EsContext (fun xx => XApp xx x2)); auto.
+ SCase "x1 hasChoice".
+ nope.
 
-   SSCase "x2 value".
-   left.
-   inverts H.
-   inverts H1.
-   inverts H2. false.
-   inverts H4.
-   exists (substXX 0 x2 x0). apply ESLamApp. auto.
+ Case "XTup".
+ assert (Forall (fun x => wnfX x \/ (exists x', STEP x x') \/ hasChoiceX x) xs) as HWS.
+ repeat nforall. rip.
+ have (exists t, TYPE ds nil nil x t). dest t.
+ have (value x \/ (exists x', STEP x x') \/ hasChoiceX x).
+ inverts H2; rip.
+ inverts H3; rip.
+ (* All ctor args are wnf, or there is a context where one can step *)
+ lets D: (@exps_ctx_run exp exp) HWS.
+ inverts D.
+ (* All ctor args are wnf *)
+ left. eauto 6.
+ (* There is a context where one ctor arg can step *)
+ right.
+ dest C. dest x'.
+ rip. destruct H3 as [STx' | HCx'].
+ left.
+ lets D: step_context_XTup_exists H1 STx'.
+ destruct D as [x'']. eauto.
+ SCase "hasChoice x".
+ nope.
 
-   SSCase "x2 steps".
-   left.
-   destruct H0 as [x2'].
-   exists (XApp x1 x2').
-   apply ESApp2; auto.
+ Case "XProj".
+ right. destruct (IHx ds); eauto.
+ SCase "value x".
+ pose proof (canonicalFormTNProd).
+ spec H0 H5. spec H0 H. dest xs; subst.
+ left.
+ pose proof (wellTypedProjHasX _ _ _ _ _ _ _ H5 H7).
+ dest x. exists x. apply EsTupProj; auto.
+ inverts H. inverts H1; auto.
+ destruct H as [STx | HCx].
+ SCase "x steps".
+ left. dest x'. exists (XProj n x').
+ eapply (EsContext (fun xx => XProj n xx)); eauto.
+ SCase "x hasChoice".
+ nope.
 
-   SSCase "x2 hasChoice".
-   inversion H0.
+ Case "XNFun".
+ left; eauto.
 
-  SCase "x1 steps".
-  left.
-  destruct H as [x1'].
-  exists (XApp x1' x2).
-  apply ESApp1; auto.
+ Case "XNApp".
+ right. destruct (IHx ds); eauto.
+ pose proof (canonicalFormTNFun).
+ spec H1 H6. spec H1 H0. dest x'; subst.
+ assert (Forall (fun x => wnfX x \/ (exists x', STEP x x') \/ hasChoiceX x) xs) as HWS.
 
-  SCase "x1 hasChoice".
-  inversion H.
+ repeat nforall. rip.
+ have (exists t, TYPE ds nil nil x t). dest t.
+ have (value x \/ (exists x', STEP x x') \/ hasChoiceX x).
+ inverts H3; rip. inverts H4. inverts H3; auto.
+ (* All args are wnf, or there is a context where one can step *)
+ lets D: (@exps_ctx_run exp exp) HWS.
+ inverts D.
+ (* All ctor args are wnf *)
+ left. eauto 6.
+ (* There is a context where one ctor arg can step *)
+ (* right. *)
+ dest C. rename x' into x''. dest x'.
+ rip. destruct H4 as [STx' | HCx'].
+ left.
+ destruct STx'.
+ exists (XNApp (XNFun ts x'') (C x)).
+ eapply (EsContext (fun xx => XNApp (XNFun ts x'') (C xx))).
+ apply XcNApp2; eauto. auto.
+ SCase "x' hasChoice".
+ nope.
+ destruct H0 as [STx | HCx].
+ left.
+ dest x'.
+ exists (XNApp x' xs); eauto.
+ eapply (EsContext (fun xx => XNApp xx xs)); eauto.
+ SCase "x hasChoice".
+ nope.
+
+ Case "XFix".
+ left; eauto.
+
+ Case "XCon".
+ (* All ctor args are either wnf or can step *)
+ assert (Forall (fun x => wnfX x \/ (exists x', STEP x x') \/ hasChoiceX x) xs) as HWS.
+ repeat nforall. rip.
+ have (exists t, TYPE ds nil nil x t). dest t.
+ have (value x \/ (exists x', STEP x x') \/ hasChoiceX x).
+ inverts H2; rip.
+ inverts H6; rip.
+ (* All ctor args are wnf, or there is a context where one can step *)
+ lets D: (@exps_ctx_run exp exp) HWS.
+ inverts D.
+ (* All ctor args are wnf *)
+ left. eauto 6.
+ (* There is a context where one ctor arg can step *)
+ right.
+ dest C. dest x'.
+ rip. destruct H6 as [STx' | HCx'].
+ left.
+ lets D: step_context_XCon_exists H1 STx'.
+ destruct D as [x'']. eauto.
+ SCase "hasChoice x".
+ nope.
+
+ Case "XMatch".
+ right.
+ destruct (IHx ds); eauto.
+ (* have HS: (value x \/ (exists x', STEP x x')). *)
+ (* inverts HS. clear IHx. *)
+ SCase "x value".
+ destruct x; nope.
+ SSCase "XCon".
+ inverts_type.
+ rewrite H8 in H9. inversion H9; subst.
+ (* rrwrite (dcs0 = dcs). *)
+ assert (exists ts x, getAlt d aa = Some (AAlt d ts x)).
+ apply getAlt_exists.
+ repeat nforall. spec H11 H15. auto.
+ (* have HG: (exists ts x, getAlt d aa = Some (AAlt d ts x)) *)
+ (*   by burn using getAlt_exists. *)
+ dest ts. dest x.
+ left. exists (substXXs 0 l x). eapply EsMatchAlt.
+ inverts H0. inverts H2; auto. eauto.
+
+ destruct H0 as [STx | HCx].
+ SCase "x steps".
+ left; destruct STx as [x'].
+ exists (XMatch x' aa).
+ lets D: EsContext XcMatch; eauto.
+ SCase "x hasChoice".
+ nope.
 Qed.
